

Schutz

7.6, The Geodesic is given by $\nabla_{\vec{p}} \vec{p} = 0$.

This is obtained by the affine reparameterization of the particle's trajectory $\vec{U}(\tau)$, where τ is the proper time.

Recall $\nabla_{\vec{U}} \vec{U} = \frac{dx^\alpha}{d\tau} V^\beta_{;\alpha} = U^\alpha V^\beta_{;\alpha}$.

under affine reparameterization $\tau \rightarrow \frac{\tau}{m}$,

$$U = \frac{dx^\alpha}{d\tau} \rightarrow \frac{dx^\alpha}{d(\tau/m)} = m \frac{dx^\alpha}{d\tau} = m \vec{U} = \vec{p}.$$

So such reparameterization $\tau \rightarrow \frac{\tau}{m}$ can be written with the original variable τ with the particle's trajectory $\vec{U}(\tau)$ replaced by $\vec{p}(\tau)$. So the geodesic equation is replaced as.

$$p^\alpha V^\beta_{;\alpha} = 0, \quad \text{for } V^\beta = p^\beta, \text{ this is } p^\alpha p^\beta_{;\alpha} = 0.$$

Schutze 7.6

Show $p^\alpha p^\beta{}_{;\alpha} = 0$ implies $p^\alpha p_\beta{}_{;\alpha} = 0$.

* The simplest proof is that $p^\beta{}_{;\alpha}$ is tensorial, so

$$p_{\beta;\alpha} = g_{\beta\sigma} p^\sigma{}_{;\alpha} \Rightarrow p^\alpha p_{\beta;\alpha} = g_{\beta\sigma} p^\alpha p^\sigma{}_{;\alpha} = 0.$$

* More sophisticated way:

$$\begin{aligned} p^\alpha p_{\beta;\alpha} &= p^\alpha \left[(g_{\beta\sigma} p^\sigma)_{;\alpha} - p_\lambda \Gamma^\lambda_{\beta\alpha} \right] \\ &= p^\alpha \left[g_{\beta\sigma;\alpha} p^\sigma + g_{\beta\sigma} p^\sigma{}_{;\alpha} - p_\lambda \frac{1}{2} g^{\lambda\omega} (g_{\beta\omega;\alpha} + g_{\alpha\omega;\beta} - g_{\alpha\beta;\omega}) \right] \\ &= p^\alpha \left[g_{\beta\sigma;\alpha} p^\sigma + g_{\beta\sigma} p^\sigma{}_{;\alpha} - \frac{1}{2} p^\sigma (g_{\beta\sigma;\alpha} + g_{\alpha\sigma;\beta} - g_{\alpha\beta;\sigma}) \right] \\ &= p^\alpha \left[p^\sigma{}_{;\alpha} g_{\beta\sigma} + p^\sigma \frac{1}{2} (g_{\beta\sigma;\alpha} + g_{\alpha\sigma;\beta} - g_{\alpha\beta;\sigma}) \right] \\ &= p^\alpha \left[p^\sigma{}_{;\alpha} g_{\beta\sigma} + p^\sigma \Gamma_{\beta\sigma\alpha} \right] \\ &= p^\alpha p^\sigma{}_{;\alpha} g_{\beta\sigma} + p^\alpha p^\sigma \Gamma_{\beta\sigma\alpha} \\ &= g_{\beta\lambda} p^\alpha p^\lambda{}_{;\alpha} + g_{\beta\lambda} \Gamma^\lambda_{\sigma\alpha} p^\alpha p^\sigma \\ &= g_{\beta\lambda} [p^\alpha] [p^\lambda{}_{;\alpha} + p^\sigma \Gamma^\lambda_{\sigma\alpha}] \\ &= \boxed{g_{\beta\lambda} p^\alpha p^\lambda{}_{;\alpha} = 0} \end{aligned}$$

Davidson Chan
7.1.2024